src/Helpers/Sets.v
@@ -31,91 +31,213 @@ Proof.
   eapply Forall_in in H; eauto.
 Qed.
 
-Inductive sorted A (lt: A -> A -> Prop) : list A -> Prop :=
-| sorted_nil : sorted lt nil
-| sorted_cons : forall x l,
-    Forall (lt x) l ->
-    sorted lt l ->
-    sorted lt (x::l).
+Lemma Forall_map : forall A (l: list A) B (f: A -> B) (P: B -> Prop),
+    Forall P (map f l) <->
+    Forall (fun x => P (f x)) l.
+Proof.
+  induction l; simpl; intuition eauto.
+  - inversion H; subst; clear H.
+    constructor; eauto.
+    apply IHl; auto.
+  - inversion H; subst; clear H.
+    constructor; eauto.
+    apply IHl; auto.
+Qed.
 
 Hint Constructors sorted.
 
 Import List.ListNotations.
 Open Scope list.
 
-Module FSet.
+Module FMap.
 
-  Section Sets.
+  Section Maps.
 
     Variable A:Type.
+    Variable V:Type.
     Context {Acmp: Ordering A}.
 
     Record t :=
-      { elements: list A;
-        elem_sorted: sorted cmp_lt elements }.
+      { elements: list (A * V);
+        keys := map fst elements;
+        elem_sorted: sorted cmp_lt keys }.
 
     Definition empty : t :=
       {| elements := [];
          elem_sorted := sorted_nil cmp_lt |}.
 
-    Definition In x (s:t) :=
-      List.In x (elements s).
+    Definition MapsTo (x:A) (v:V) (s:t) :=
+      List.In (x, v) (elements s).
+
+    Definition In (x:A) (s:t) :=
+      List.In x (keys s).
+
+    Theorem empty_mapsto : forall x v,
+        ~MapsTo x v empty.
+    Proof.
+      compute; auto.
+    Qed.
 
     Theorem empty_in : forall x,
         ~In x empty.
     Proof.
-      unfold In, empty; simpl; eauto.
+      compute; eauto.
     Qed.
 
-    Definition For_all (P:A -> Prop) (s:t) :=
+    Lemma cmp_lt_irrefl : forall x,
+        cmp_lt x x -> False.
+    Proof.
+      unfold cmp_lt; intros.
+      rewrite cmp_refl in *; congruence.
+    Qed.
+
+    Hint Resolve cmp_lt_irrefl.
+
+    Ltac forall_in :=
+      match goal with
+      | [ H: Forall ?P ?l, H': List.In ?x ?l |- _ ] =>
+        let Hnew := fresh in
+        pose proof (Forall_in H _ H') as Hnew;
+        clear H';
+        simpl in Hnew
+      end.
+
+    Lemma all_keys_lt : forall (l: list (A*V)) (x:A),
+        Forall (cmp_lt x) (map fst l) ->
+        forall v, ~List.In (x, v) l.
+    Proof.
+      unfold not; intros.
+      apply -> Forall_map in H.
+      forall_in.
+      exfalso; eauto.
+    Qed.
+
+    Theorem mapsto_unique : forall x v v' m,
+        MapsTo x v m ->
+        MapsTo x v' m ->
+        v = v'.
+    Proof.
+      unfold MapsTo; intros.
+      pose proof (elem_sorted m).
+      unfold keys in *.
+      generalize dependent (elements m); clear m.
+      induction l; simpl in *; intros; eauto.
+      - exfalso; auto.
+      - destruct a as [x' v'']; simpl in *.
+        inversion_clear H1.
+        intuition (subst; eauto);
+          repeat match goal with
+                 | [ H: (_, _) = (_, _) |- _ ] =>
+                   inversion H; subst; clear H
+                 end;
+          auto.
+        exfalso; eapply all_keys_lt; eauto.
+        exfalso; eapply all_keys_lt; eauto.
+    Qed.
+
+    Definition For_all (P:A*V -> Prop) (s:t) :=
       Forall P (elements s).
 
     Theorem empty_Forall : forall P,
         For_all P empty.
     Proof.
-      unfold For_all; simpl; eauto.
+      compute; eauto.
     Qed.
 
-    Theorem For_all_in (P:A -> Prop) (s:t) :
+    Theorem For_all_in (P:A*V -> Prop) (s:t) :
       For_all P s ->
-      forall x, In x s -> P x.
+      forall x v, MapsTo x v s -> P (x, v).
     Proof.
-      unfold For_all, In; simpl; intros.
+      unfold For_all, MapsTo; simpl; intros.
       eapply Forall_in; eauto.
     Qed.
 
     Theorem not_in_forall : forall x s,
         ~In x s ->
-        For_all (fun y => x <> y) s.
+        For_all (fun y => x <> fst y) s.
     Proof.
       unfold In, For_all.
       destruct s; simpl; intros.
+      unfold keys in *; simpl in *.
       clear elem_sorted0.
       induction elements0; simpl in *; eauto 10.
     Qed.
 
     Definition In_dec x s : {In x s} + {~In x s}.
       unfold In.
-      destruct (List.in_dec cmp_dec x (elements s)); eauto.
+      apply (List.in_dec cmp_dec x (keys s)).
     Defined.
 
-    Fixpoint _add (x0:A) (l:list A) : list A :=
+    Fixpoint _add (x0:A) (v0:V) (l:list (A*V)) : list (A*V) :=
+      match l with
+      | nil => (x0,v0)::nil
+      | (x,v)::xs => match cmp x0 x with
+                    | Lt => (* x0 can go at the very beginning*)
+                      (x0,v0)::l
+                    | Gt => (* x0 should go later *)
+                      (x,v)::_add x0 v0 xs
+                    | Eq => (* x0 is already in the list *)
+                      (x,v0)::xs
+                    end
+      end.
+
+    Fixpoint _add_key (x0:A) (l:list A) : list A :=
       match l with
       | nil => x0::nil
       | x::xs => match cmp x0 x with
-                | Lt => (* x0 can go at the very beginning*)
-                  x0::l
-                | Gt => (* x0 should go later *)
-                  x::_add x0 xs
-                | Eq => (* x0 is already in the list *)
-                  l
-                end
+                    | Lt => (* x0 can go at the very beginning*)
+                      x0::l
+                    | Gt => (* x0 should go later *)
+                      x::_add_key x0 xs
+                    | Eq => (* x0 is already in the list *)
+                      l
+                    end
       end.
 
-    Theorem _add_forall : forall x P l,
+    Theorem _add_key_keys : forall x v (l: list (A*V)),
+        map fst (_add x v l) = _add_key x (map fst l).
+    Proof.
+      induction l; simpl; auto.
+      destruct a; simpl.
+      destruct (cmp x a); simpl; auto.
+      congruence.
+    Qed.
+
+    Theorem _add_forall : forall x v P l,
+        Forall P l ->
+        P (x, v) ->
+        Forall P (_add x v l).
+    Proof.
+      induction l; simpl; intros; eauto.
+      inversion H; subst; clear H.
+      destruct a as [x' v'].
+      destruct (ord_spec x x');
+        (intuition subst); eauto.
+    Qed.
+
+    Hint Resolve _add_forall.
+
+    Theorem _add_forall' : forall x v P l,
+        ~List.In x (map fst l) ->
+        Forall P (_add x v l) ->
+        Forall P l.
+    Proof.
+      induction l; simpl; intros; eauto.
+      destruct a as [x' v'].
+      destruct (ord_spec x x');
+        simpl in *;
+        intuition subst.
+      - congruence.
+      - rewrite H2 in *.
+        inversion H0; eauto.
+      - rewrite H3 in *.
+        inversion H0; eauto.
+    Qed.
+
+    Theorem _add_key_forall : forall x P l,
         Forall P l ->
         P x ->
-        Forall P (_add x l).
+        Forall P (_add_key x l).
     Proof.
       induction l; simpl; intros; eauto.
       inversion H; subst; clear H.
@@ -123,130 +245,159 @@ Module FSet.
         (intuition subst); eauto.
     Qed.
 
-    Hint Resolve _add_forall.
+    Hint Resolve _add_key_forall.
 
-    Theorem _add_forall' : forall x P l,
-        Forall P (_add x l) ->
-        Forall P l.
+    Theorem _add_respectful : forall x v l,
+        sorted cmp_lt (map fst l) ->
+        sorted cmp_lt (map fst (_add x v l)).
     Proof.
-      induction l; simpl; intros; eauto.
-      destruct (ord_spec x a);
-        intuition subst.
-      - rewrite cmp_refl in H; auto.
-      - rewrite H1 in *.
-        inversion H; eauto.
-      - rewrite H2 in *.
-        inversion H; eauto.
-    Qed.
-
-    Theorem _add_respectful : forall x l,
-        sorted cmp_lt l ->
-        sorted cmp_lt (_add x l).
-    Proof.
+      intros.
+      rewrite _add_key_keys.
+      generalize dependent (map fst l); clear l.
       induction 1; simpl; eauto.
       destruct (ord_spec x x0); intuition subst.
       - eauto.
       - constructor; eauto.
         constructor; eauto.
-        eapply Forall_impl. 2: eauto.
+        eapply Forall_impl; [ | eauto ].
         intros.
         eapply cmp_trans; eauto.
       - constructor; eauto.
     Qed.
 
-    Definition add (x:A) (s:t) : t :=
-      {| elements := _add x (elements s);
-         elem_sorted := _add_respectful x (elem_sorted s); |}.
+    Definition add (x:A) (v:V) (s:t) : t :=
+      {| elements := _add x v (elements s);
+         elem_sorted := _add_respectful
+                          x v (elements s) (elem_sorted s); |}.
 
-    Theorem add_forall : forall x P s,
+    Theorem add_forall : forall x v P s,
         For_all P s ->
-        P x ->
-        For_all P (add x s).
+        P (x, v) ->
+        For_all P (add x v s).
     Proof.
       unfold For_all, add; simpl; intros.
       eapply _add_forall; eauto.
     Qed.
 
-    Theorem add_forall' : forall x P s,
-        For_all P (add x s) ->
+    Theorem add_forall' : forall x v P s,
+        ~In x s ->
+        For_all P (add x v s) ->
         For_all P s.
     Proof.
       unfold For_all, add; simpl; intros.
       eapply _add_forall'; eauto.
     Qed.
 
-    Theorem _add_in : forall x l,
-        List.In x (_add x l).
+    Theorem _add_mapsto : forall x v l,
+        List.In (x, v) (_add x v l).
     Proof.
       induction l; simpl; eauto.
-      destruct (ord_spec x a); simpl; eauto.
+      destruct a as [x' v'].
+      destruct (ord_spec x x'); subst; simpl; eauto.
     Qed.
 
-    Theorem add_in : forall x s,
-        In x (add x s).
+    Theorem _add_in : forall x v l,
+        List.In x (map fst (_add x v l)).
+    Proof.
+      induction l; simpl; eauto.
+      destruct a as [x' v'].
+      destruct (ord_spec x x'); subst; simpl; eauto.
+    Qed.
+
+    Theorem add_mapsto : forall x v s,
+        MapsTo x v (add x v s).
+    Proof.
+      unfold add, MapsTo; simpl.
+      unfold keys; simpl; intros.
+      eapply _add_mapsto.
+    Qed.
+
+    Theorem add_in : forall x v s,
+        In x (add x v s).
     Proof.
       unfold add, In; simpl.
-      eauto using _add_in.
+      unfold keys; simpl; intros.
+      eapply _add_in.
     Qed.
 
-    Theorem add_in' : forall x s y,
-        In x (add y s) ->
+    Theorem add_in' : forall x s y v,
+        In x (add y v s) ->
         x = y \/ In x s.
     Proof.
       destruct s as [s H].
       unfold In, add; simpl; intros.
       induction s; simpl in *; intuition eauto.
-      inversion H; subst; clear H; intuition auto.
-      destruct (ord_spec y a); subst; intuition.
+      subst H.
+      compute [keys elements] in *.
+      destruct a as [y' v'].
+      inversion elem_sorted0; subst; clear elem_sorted0; intuition auto.
+      destruct (ord_spec y y'); subst; intuition.
       - rewrite cmp_refl in *.
         simpl in *; intuition auto.
-      - rewrite H2 in *.
+      - rewrite H4 in *; intuition eauto.
         simpl in *; intuition auto.
       - rewrite H5 in *.
         simpl in *; intuition auto.
     Qed.
 
-    Theorem _add_incr : forall x l y,
-        List.In y l ->
-        List.In y (_add x l).
-    Proof.
-      induction l; simpl; intros; eauto.
-      destruct (ord_spec x a); simpl; intuition eauto.
-    Qed.
+    Fixpoint _remove (x0:A) (l:list (A*V)) : list (A*V) :=
+      match l with
+      | nil => nil
+      | (x,v)::xs => match cmp x0 x with
+                | Lt => l
+                | Eq => xs
+                | Gt => (x,v)::_remove x0 xs
+                end
+      end.
 
-    Theorem add_incr : forall x s y,
-        In y s ->
-        In y (add x s).
-    Proof.
-      unfold add, In; simpl.
-      eauto using _add_incr.
-    Qed.
-
-    Fixpoint _remove (x0:A) (l:list A) : list A :=
+    Fixpoint _remove_key (x0:A) (l:list A) : list A :=
       match l with
       | nil => nil
       | x::xs => match cmp x0 x with
                 | Lt => l
                 | Eq => xs
-                | Gt => x::_remove x0 xs
+                | Gt => x::_remove_key x0 xs
                 end
       end.
+
+    Theorem _remove_key_keys : forall x (l: list (A*V)),
+        map fst (_remove x l) = _remove_key x (map fst l).
+    Proof.
+      induction l; simpl; auto.
+      destruct a as [x' v]; simpl.
+      destruct (cmp x x'); simpl; congruence.
+    Qed.
 
     Theorem _remove_forall : forall x P l,
         Forall P l ->
         Forall P (_remove x l).
     Proof.
       induction 1; simpl; eauto.
-      destruct (ord_spec x x0);
+      destruct x0 as [x' v].
+      destruct (ord_spec x x');
         subst; eauto.
     Qed.
 
     Hint Resolve _remove_forall.
 
-    Theorem _remove_respectful : forall x l,
-        sorted cmp_lt l ->
-        sorted cmp_lt (_remove x l).
+    Theorem _remove_key_forall : forall x P l,
+        Forall P l ->
+        Forall P (_remove_key x l).
     Proof.
+      induction 1; simpl; eauto.
+      destruct (ord_spec x x0);
+        subst; eauto.
+    Qed.
+
+    Hint Resolve _remove_key_forall.
+
+    Theorem _remove_respectful : forall x l,
+        sorted cmp_lt (map fst l) ->
+        sorted cmp_lt (map fst (_remove x l)).
+    Proof.
+      intros.
+      rewrite _remove_key_keys.
+      generalize dependent (map fst l); clear l.
       induction l; simpl; intros; eauto.
       inversion H; subst; clear H.
       destruct (ord_spec x a);
@@ -256,7 +407,8 @@ Module FSet.
 
     Definition remove x (s:t) : t :=
       {| elements := _remove x (elements s);
-         elem_sorted := _remove_respectful x (elem_sorted s); |}.
+         elem_sorted := _remove_respectful
+                          x (elements s) (elem_sorted s); |}.
 
     Lemma forall_lt_not_in : forall x l,
         Forall (cmp_lt x) l ->
@@ -264,19 +416,11 @@ Module FSet.
     Proof.
       unfold not, cmp_lt; intros.
       eapply Forall_in in H; eauto.
-      rewrite cmp_refl in H; congruence.
     Qed.
-
-    Ltac forall_in :=
-      match goal with
-      | [ H: Forall ?P ?l, H': List.In ?x ?l |- _ ] =>
-        pose proof (Forall_in H _ H');
-        clear H'
-      end.
 
     Theorem _remove_not_in : forall x l,
         sorted cmp_lt l ->
-        ~List.In x (_remove x l).
+        ~List.In x (_remove_key x l).
     Proof.
       unfold not; intros.
       induction l; simpl in *; eauto.
@@ -298,15 +442,32 @@ Module FSet.
     Theorem remove_not_in : forall x s,
         ~In x (remove x s).
     Proof.
-      unfold In, remove; simpl; intros.
+      unfold In, remove, keys; simpl; intros.
+      rewrite _remove_key_keys.
       eapply _remove_not_in.
       apply (elem_sorted s).
+    Qed.
+
+    Theorem _remove_mapsto : forall x l y v,
+        List.In (y, v) l ->
+        x <> y ->
+        List.In (y, v) (_remove x l).
+    Proof.
+      induction l; simpl; intuition subst.
+      - inversion_clear H1.
+        destruct (ord_spec x y);
+          simpl;
+          (intuition subst).
+      - destruct (ord_spec x a0);
+          simpl;
+          (intuition subst).
+        eauto.
     Qed.
 
     Theorem _remove_in : forall x l y,
         List.In y l ->
         x <> y ->
-        List.In y (_remove x l).
+        List.In y (_remove_key x l).
     Proof.
       induction l; simpl; intuition subst.
       - destruct (ord_spec x y);
@@ -318,12 +479,22 @@ Module FSet.
         eauto.
     Qed.
 
+    Theorem remove_mapsto : forall x s y v,
+        MapsTo y v s ->
+        x <> y ->
+        MapsTo y v (remove x s).
+    Proof.
+      unfold MapsTo, remove, keys; simpl; intros.
+      auto using _remove_mapsto.
+    Qed.
+
     Theorem remove_in : forall x s y,
         In y s ->
         x <> y ->
         In y (remove x s).
     Proof.
-      unfold In, remove; simpl; intros.
+      unfold In, remove, keys; simpl; intros.
+      rewrite _remove_key_keys.
       auto using _remove_in.
     Qed.
 
@@ -332,27 +503,26 @@ Module FSet.
         In x s /\ x <> y.
     Proof.
       destruct s as [s H].
-      unfold In, remove; simpl; intros.
+      unfold In, remove, keys; simpl; intros.
       induction s; simpl in *; eauto.
-      destruct (ord_spec y a); subst.
+      destruct a as [y' v'].
+      subst H; simpl in *.
+      destruct (ord_spec y y'); subst.
       - rewrite cmp_refl in *.
-        inversion H; subst; clear H; intuition (subst; auto).
-        eapply Forall_in in H3; eauto.
-        unfold cmp_lt in *; rewrite cmp_refl in *; congruence.
-      - destruct H1.
-        rewrite H1 in *.
-        simpl in *.
+        inversion elem_sorted0; subst; clear elem_sorted0;
+          intuition (subst; auto).
+        eapply Forall_in in H2; eauto.
+      - destruct H.
+        rewrite H in *; simpl in *.
         intuition (subst; eauto).
-        rewrite cmp_refl in *; congruence.
-        inversion H; subst; clear H; intuition eauto.
-        eapply Forall_in in H3; eauto.
-        congruence.
-      - destruct H1.
-        rewrite H2 in *.
-        simpl in *; intuition (subst; eauto).
-        rewrite cmp_refl in *; congruence.
-        inversion H; subst; clear H; intuition eauto.
-        inversion H; subst; clear H; intuition eauto.
+        inversion elem_sorted0; subst; clear elem_sorted0;
+          intuition eauto.
+        forall_in; congruence.
+      - destruct H.
+        rewrite H1 in *; simpl in *.
+        intuition (subst; eauto).
+        inversion_clear elem_sorted0; intuition eauto.
+        inversion_clear elem_sorted0; intuition eauto.
     Qed.
 
     Lemma cmp_lt_antisym : forall x y,
@@ -364,66 +534,115 @@ Module FSet.
       apply cmp_antisym in H; congruence.
     Qed.
 
-    Theorem set_extensionality : forall s1 s2,
-        (forall x, In x s1 <-> In x s2) ->
+    Theorem mapsto_extensionality : forall s1 s2,
+        (forall x v, MapsTo x v s1 <-> MapsTo x v s2) ->
         s1 = s2.
     Proof.
       unfold In; intros.
-      destruct s1 as [s1 s1_sorted].
-      destruct s2 as [s2 s2_sorted].
-      simpl in *.
+      destruct s1 as [s1 ? s1_sorted].
+      destruct s2 as [s2 ? s2_sorted].
+      subst keys0 keys1.
+      unfold MapsTo, keys in *; simpl in *.
       assert (s1 = s2).
       generalize dependent H.
       generalize dependent s2_sorted.
       generalize dependent s1_sorted.
       eapply two_list_induction with (l1:=s1) (l2:=s2);
         simpl; intros; eauto.
+      destruct y as [x v].
       exfalso; eapply H; eauto.
+      destruct x as [x v].
       exfalso; eapply H; eauto.
       inversion s1_sorted; subst; clear s1_sorted.
       inversion s2_sorted; subst; clear s2_sorted.
+      intuition idtac.
 
-      assert (~List.In x xs) by eauto using forall_lt_not_in.
-      assert (~List.In y ys) by eauto using forall_lt_not_in.
+      destruct x as [x v1].
+      destruct y as [y v2].
+      simpl in *.
+      assert (~List.In (x, v1) xs) by eauto using all_keys_lt.
+      assert (~List.In (y, v2) ys) by eauto using all_keys_lt.
 
-      assert (x = y). {
-        pose proof (H0 x).
-        pose proof (H0 y).
-        intuition eauto.
+      assert (x = y /\ v1 = v2). {
+        pose proof (H0 x v1).
+        pose proof (H0 y v2).
+        apply -> Forall_map in H3.
+        apply -> Forall_map in H5.
+        (intuition eauto);
+          repeat match goal with
+                 | [ H: (_, _) = (_, _) |- _ ] =>
+                   inversion H; subst; clear H
+                 end;
+          intuition idtac.
         repeat forall_in.
         exfalso; eauto using cmp_lt_antisym.
-      } subst; f_equal.
+        repeat forall_in.
+        exfalso; eauto using cmp_lt_antisym.
+      } intuition subst; f_equal.
       eapply H; eauto.
       intros.
-      specialize (H0 x).
-      intuition (subst; eauto);
-        try solve [ exfalso; eauto using forall_lt_not_in ].
+      pose proof (H0 x v).
+      apply -> Forall_map in H3.
+      apply -> Forall_map in H5.
+      (intuition eauto);
+        repeat match goal with
+               | [ H: (_, _) = (_, _) |- _ ] =>
+                 inversion H; subst; clear H
+               end;
+        intuition idtac.
       destruct H0.
       f_equal.
       apply proof_irrelevance.
     Qed.
 
-    Fixpoint _filter (P: A -> bool) (l: list A) : list A :=
+    Fixpoint _filter (P: A -> bool) (l: list (A*V)) : list (A*V) :=
       match l with
       | [] => []
-      | x::xs => if P x then x::_filter P xs
+      | (x,v)::xs => if P x then (x,v)::_filter P xs
                 else _filter P xs
       end.
 
+    Fixpoint _filter_key (P: A -> bool) (l: list A) : list A :=
+      match l with
+      | [] => []
+      | x::xs => if P x then x::_filter_key P xs
+                else _filter_key P xs
+      end.
+
+    Theorem _filter_key_keys : forall P l,
+        map fst (_filter P l) = _filter_key P (map fst l).
+    Proof.
+      induction l; simpl; auto.
+      destruct a as [x v]; simpl.
+      destruct (P x); simpl; congruence.
+    Qed.
+
     Theorem _filter_in : forall P l,
-        forall x, List.In x (_filter P l) ->
+        forall x v, List.In (x, v) (_filter P l) ->
+               List.In (x, v) l.
+    Proof.
+      induction l; simpl; intros; auto.
+      destruct a as [x' v'].
+      destruct (P x'); simpl in *; intuition eauto.
+    Qed.
+
+    Theorem _filter_key_in : forall P l,
+        forall x, List.In x (_filter_key P l) ->
              List.In x l.
     Proof.
       induction l; simpl; intros; auto.
       destruct (P a); simpl in *; intuition eauto.
     Qed.
 
-    Hint Resolve _filter_in.
+    Hint Resolve _filter_key_in.
 
     Theorem _filter_respectful : forall P l,
-        sorted cmp_lt l ->
-        sorted cmp_lt (_filter P l).
+        sorted cmp_lt (map fst l) ->
+        sorted cmp_lt (map fst (_filter P l)).
     Proof.
+      intros.
+      rewrite _filter_key_keys.
+      generalize dependent (map fst l); clear l.
       induction l; simpl; intros; auto.
       inversion H; subst; intuition eauto.
       destruct (P a); eauto.
@@ -441,19 +660,22 @@ Module FSet.
         In x (filter P s) ->
         In x s.
     Proof.
-      unfold In, filter; simpl; intros.
+      unfold In, filter, keys; simpl; intros.
+      rewrite _filter_key_keys in *.
       eauto using _filter_in.
     Qed.
 
     Theorem filter_spec : forall P s,
-        For_all (fun y => P y = true) (filter P s).
+        For_all (fun '(x, _) => P x = true) (filter P s).
     Proof.
       unfold For_all, filter.
       destruct s as [s H].
       simpl.
+      subst H.
       induction s; simpl; intros; auto.
-      inversion H; subst; clear H; intuition.
-      destruct_with_eqn (P a); eauto.
+      destruct a as [x v]; simpl in *.
+      inversion elem_sorted0; subst; clear elem_sorted0; intuition.
+      destruct_with_eqn (P x); eauto.
     Qed.
 
     Theorem filter_complete : forall P s x,
@@ -462,18 +684,20 @@ Module FSet.
         In x (filter P s).
     Proof.
       destruct s as [s H].
-      unfold In, filter; simpl; intros.
+      unfold In, filter, keys; simpl; intros.
+      subst H.
       induction s; simpl; intros; auto.
-      inversion H; subst; clear H; intuition.
-      simpl in H0.
-      destruct_with_eqn (P a); simpl; intuition eauto.
-      subst; eauto.
-      congruence.
+      destruct a as [x' v']; simpl in *.
+      inversion elem_sorted0; subst; clear elem_sorted0; intuition.
+      - subst.
+        destruct_with_eqn (P x); simpl; intuition eauto.
+        congruence.
+      - destruct_with_eqn (P x'); simpl; intuition eauto.
     Qed.
 
-  End Sets.
+  End Maps.
 
-  Arguments t A {Acmp}.
-  Arguments empty {A} {Acmp}.
+  Arguments t A V {Acmp}.
+  Arguments empty {A} {V} {Acmp}.
 
-End FSet.
+End FMap.
